src/hls/AssocMap.v
@@ -252,15 +252,15 @@ Notation "a # b '<-' c" := (AssocMap.set b c a) (at level 1, b at next level) : 
 
 Local Open Scope assocmap.
 Lemma find_get_assocmap :
-  forall assoc r v,
+  forall n assoc r v,
   assoc ! r = Some v ->
-  assoc # r = v.
+  find_assocmap n r assoc = v.
 Proof. intros. unfold find_assocmap, AssocMapExt.get_default. rewrite H. trivial. Qed.
 
 Lemma merge_get_default :
-  forall ars ars' r x,
+  forall n ars ars' r x,
     ars ! r = Some x ->
-    (AssocMapExt.merge _ ars ars') # r = x.
+    find_assocmap n r (AssocMapExt.merge _ ars ars') = x.
 Proof.
   unfold AssocMapExt.merge; intros.
   unfold "#", AssocMapExt.get_default.
@@ -270,9 +270,9 @@ Proof.
 Qed.
 
 Lemma merge_get_default2 :
-  forall ars ars' r,
+  forall n ars ars' r,
     ars ! r = None ->
-    (AssocMapExt.merge _ ars ars') # r = ars' # r.
+    find_assocmap n r (AssocMapExt.merge _ ars ars') = find_assocmap n r ars'.
 Proof.
   unfold AssocMapExt.merge; intros.
   unfold "#", AssocMapExt.get_default.
@@ -323,4 +323,21 @@ Proof.
   unfold AssocMapExt.merge; intros.
   rewrite ! AssocMap.gcombine by auto.
   now rewrite AssocMap.gso by auto.
+Qed.
+
+Lemma assocmap_gso :
+  forall n a a' c b,
+    a <> a' ->
+    find_assocmap n a (AssocMap.set a' c b) = find_assocmap n a b.
+Proof.
+  intros. unfold find_assocmap, AssocMapExt.get_default.
+  now rewrite AssocMap.gso by auto.
+Qed.
+
+Lemma assocmap_gss :
+  forall n a c b,
+    find_assocmap n a (AssocMap.set a c b) = c.
+Proof.
+  intros. unfold find_assocmap, AssocMapExt.get_default.
+  now rewrite AssocMap.gss by auto.
 Qed.
