src/hls/ClockMemory.v
@@ -1,0 +1,79 @@
+(*
+ * Vericert: Verified high-level synthesis.
+ * Copyright (C) 2023 Yann Herklotz <yann@yannherklotz.com>
+ *
+ * This program is free software: you can redistribute it and/or modify
+ * it under the terms of the GNU General Public License as published by
+ * the Free Software Foundation, either version 3 of the License, or
+ * (at your option) any later version.
+ *
+ * This program is distributed in the hope that it will be useful,
+ * but WITHOUT ANY WARRANTY; without even the implied warranty of
+ * MERCHANTABILITY or FITNESS FOR A PARTICULAR PURPOSE.  See the
+ * GNU General Public License for more details.
+ *
+ * You should have received a copy of the GNU General Public License
+ * along with this program.  If not, see <https://www.gnu.org/licenses/>.
+ *)
+
+Require Import Coq.FSets.FMapPositive.
+Require Import Coq.micromega.Lia.
+
+Require compcert.common.Events.
+Require compcert.common.Globalenvs.
+Require compcert.common.Smallstep.
+Require compcert.common.Values.
+Require Import compcert.lib.Integers.
+Require Import compcert.lib.Maps.
+Require Import compcert.common.AST.
+
+Require Import vericert.common.Vericertlib.
+Require Import vericert.hls.ValueInt.
+Require Import vericert.hls.AssocMap.
+Require Import vericert.hls.Array.
+Require Import vericert.common.Monad.
+Require Import vericert.common.Optionmonad.
+Require Import vericert.hls.Verilog.
+Require Import vericert.hls.DHTL.
+
+Import OptionExtra.
+
+#[local] Open Scope monad_scope.
+
+Definition pred := positive.
+
+Definition transf_maps (d: stmnt) :=
+  match d with
+  | Vseq ((Vblock (Vvar _) _) as rest) (Vblock (Vvari r e1) e2) =>
+    Vseq rest (Vnonblock (Vvari r e1) e2)
+  | Vseq (Vblock (Vvar st') e3) (Vblock (Vvar e1) (Vvari r e2)) =>
+    Vseq (Vblock (Vvar st') e3) (Vnonblock (Vvar e1) (Vvari r e2))
+  | _ => d
+  end.
+
+Program Definition transf_module (m: DHTL.module) : DHTL.module :=
+  mkmodule m.(mod_params)
+      (PTree.map1 transf_maps m.(mod_datapath))
+      m.(mod_entrypoint)
+      m.(mod_st)
+      m.(mod_stk)
+      m.(mod_stk_len)
+      m.(mod_finish)
+      m.(mod_return)
+      m.(mod_start)
+      m.(mod_reset)
+      m.(mod_clk)
+      m.(mod_scldecls)
+      m.(mod_arrdecls)
+      m.(mod_ram) 
+      _
+      m.(mod_ordering_wf)
+      m.(mod_ram_wf)
+      m.(mod_params_wf).
+Next Obligation.
+Admitted.
+
+Definition transf_fundef := transf_fundef transf_module.
+
+Definition transf_program (p : DHTL.program) : DHTL.program :=
+  transform_program transf_fundef p.
